syntax.v
@@ -1,0 +1,35 @@
+Inductive ty : Type :=
+| TBool : ty
+| TNat : ty
+| TList : ty -> ty.
+
+(* Intrinsically typed expression syntax *)
+Inductive exp : list ty -> ty -> Type :=
+| evar : forall G t, member t G -> exp G t
+| etrue : forall G, exp G TBool
+| efalse : forall G, exp G TBool
+| econst : forall G, nat -> exp G TNat
+| eplus : forall G, exp G TNat -> exp G TNat -> exp G TNat
+| enil : forall G t, exp G (TList t)
+| econs : forall G t, exp G t -> exp G (TList t) -> exp G (TList t)
+| elet : forall G t1 t2, exp G t1 -> exp (t1 :: G) t2 -> exp G t2
+| eappend : forall G t, exp G (TList t) -> exp G (TList t) -> exp G (TList t)
+| emap : forall G t1 t2, exp (t1 :: G) t2 -> exp G (TList t1) ->exp G (TList t2).
+
+Arguments econst [G].
+Arguments etrue [G].
+Arguments efalse [G].
+Arguments enil [G t].
+
+Notation "[| |]" := enil.
+Notation "[| x |]" := (econs x nil).
+Notation "[| x ; y ; .. ; z |]" := (econs x (econs y .. (econs z enil) ..)).
+Notation "[| x ; .. ; y |]" := (econs x .. (econs y enil) ..).
+
+(* Intrinsically typed values as well *)
+Inductive val : ty -> Type :=
+| vtrue : val TBool
+| vfalse : val TBool
+| vconst : nat -> val TNat
+| vnil : forall t, val (TList t)
+| vcons : forall t, val t -> val (TList t) -> val (TList t).
